iris/base_logic/lib/mono_Z.v
@@ -2,7 +2,7 @@
 This is basically a [Z]-typed wrapper over [mono_nat], which can be useful when
 one wants to use [Z] consistently for everything.
 Provides an authoritative proposition [mono_Z_auth_own γ q n] for the
-underlying number [n] and a persistent proposition [mono_nat_lb_own γ m]
+underlying number [n] and a persistent proposition [mono_Z_lb_own γ m]
 witnessing that the authoritative nat is at least [m].
 
 The key rules are [mono_Z_lb_own_valid], which asserts that an auth at [n] and
@@ -29,22 +29,33 @@ Class mono_ZG Σ :=
 Definition mono_ZΣ := mono_natΣ.
 
 Local Definition mono_Z_auth_own_def `{!mono_ZG Σ}
-    (γ : gname) (q : Qp) (n : Z) : iProp Σ :=
-  ⌜0 ≤ n⌝ ∗ mono_nat_auth_own γ q (Z.to_nat n).
+    (γ : gname) (dq : dfrac) (n : Z) : iProp Σ :=
+  ⌜0 ≤ n⌝ ∗ γ ↪●MN{dq} (Z.to_nat n).
 Local Definition mono_Z_auth_own_aux : seal (@mono_Z_auth_own_def).
 Proof. by eexists. Qed.
 Definition mono_Z_auth_own := mono_Z_auth_own_aux.(unseal).
 Local Definition mono_Z_auth_own_unseal :
   @mono_Z_auth_own = @mono_Z_auth_own_def := mono_Z_auth_own_aux.(seal_eq).
-Global Arguments mono_Z_auth_own {Σ _} γ q n.
+Global Arguments mono_Z_auth_own {Σ _} γ dq n.
 
 Local Definition mono_Z_lb_own_def `{!mono_ZG Σ} (γ : gname) (n : Z) : iProp Σ :=
-  ⌜0 ≤ n⌝ ∗ mono_nat_lb_own γ (Z.to_nat n).
+  ⌜0 ≤ n⌝ ∗ γ ↪◯MN (Z.to_nat n).
 Local Definition mono_Z_lb_own_aux : seal (@mono_Z_lb_own_def). Proof. by eexists. Qed.
 Definition mono_Z_lb_own := mono_Z_lb_own_aux.(unseal).
 Local Definition mono_Z_lb_own_unseal :
   @mono_Z_lb_own = @mono_Z_lb_own_def := mono_Z_lb_own_aux.(seal_eq).
 Global Arguments mono_Z_lb_own {Σ _} γ n.
+
+Notation "γ ↪●MZ dq n" := (mono_Z_auth_own γ dq n)
+  (at level 20, dq custom dfrac at level 1,
+   format "γ  ↪●MZ dq  n").
+Notation "γ ↪◯MZ n" := (mono_Z_lb_own γ n)
+  (at level 20).
+
+(* Compatibility alias. Do not use for new code.
+This will eventually be deprecated and removed. *)
+Notation mono_Z_auth_own_frac γ q n :=
+  (mono_Z_auth_own γ (DfracOwn q) n) (only parsing).
 
 Local Ltac unseal := rewrite
   ?mono_Z_auth_own_unseal /mono_Z_auth_own_def
@@ -54,42 +65,44 @@ Section mono_Z.
   Context `{!mono_ZG Σ}.
   Implicit Types (n m : Z).
 
-  Global Instance mono_Z_auth_own_timeless γ q n : Timeless (mono_Z_auth_own γ q n).
+  Global Instance mono_Z_auth_own_timeless γ dq n : Timeless (γ ↪●MZ{dq} n).
   Proof. unseal. apply _. Qed.
-  Global Instance mono_Z_lb_own_timeless γ n : Timeless (mono_Z_lb_own γ n).
+  Global Instance mono_Z_auth_own_persistent γ n : Persistent (γ ↪●MZ□ n).
   Proof. unseal. apply _. Qed.
-  Global Instance mono_Z_lb_own_persistent γ n : Persistent (mono_Z_lb_own γ n).
+  Global Instance mono_Z_lb_own_timeless γ n : Timeless (γ ↪◯MZ n).
+  Proof. unseal. apply _. Qed.
+  Global Instance mono_Z_lb_own_persistent γ n : Persistent (γ ↪◯MZ n).
   Proof. unseal. apply _. Qed.
 
   Global Instance mono_Z_auth_own_fractional γ n :
-    Fractional (λ q, mono_Z_auth_own γ q n).
+    Fractional (λ q, γ ↪●MZ{#q} n).
   Proof.
     unseal. intros p q. iSplit.
     - iIntros "[% [$ $]]". eauto.
     - iIntros "[[% H1] [% H2]]". iCombine "H1 H2" as "$". eauto.
   Qed.
   Global Instance mono_Z_auth_own_as_fractional γ q n :
-    AsFractional (mono_Z_auth_own γ q n) (λ q, mono_Z_auth_own γ q n) q.
+    AsFractional (γ ↪●MZ{#q} n) (λ q, γ ↪●MZ{#q} n) q.
   Proof. split; [auto|apply _]. Qed.
 
-  Lemma mono_Z_auth_own_agree γ q1 q2 n1 n2 :
-    mono_Z_auth_own γ q1 n1 -∗
-    mono_Z_auth_own γ q2 n2 -∗
-    ⌜(q1 + q2 ≤ 1)%Qp ∧ n1 = n2⌝.
+  Lemma mono_Z_auth_own_agree γ dq1 dq2 n1 n2 :
+    γ ↪●MZ{dq1} n1 -∗
+    γ ↪●MZ{dq2} n2 -∗
+    ⌜✓ (dq1 ⋅ dq2) ∧ n1 = n2⌝.
   Proof.
     unseal. iIntros "[% H1] [% H2]".
     iDestruct (mono_nat_auth_own_agree with "H1 H2") as %?.
     iPureIntro. naive_solver lia.
   Qed.
   Lemma mono_Z_auth_own_exclusive γ n1 n2 :
-    mono_Z_auth_own γ 1 n1 -∗ mono_Z_auth_own γ 1 n2 -∗ False.
+    γ ↪●MZ n1 -∗ γ ↪●MZ n2 -∗ False.
   Proof.
     iIntros "H1 H2".
     by iDestruct (mono_Z_auth_own_agree with "H1 H2") as %[[] _].
   Qed.
 
-  Lemma mono_Z_lb_own_valid γ q n m :
-    mono_Z_auth_own γ q n -∗ mono_Z_lb_own γ m -∗ ⌜(q ≤ 1)%Qp ∧ m ≤ n⌝.
+  Lemma mono_Z_lb_own_valid γ dq n m :
+    γ ↪●MZ{dq} n -∗ γ ↪◯MZ m -∗ ⌜✓ dq ∧ m ≤ n⌝.
   Proof.
     unseal. iIntros "[% Hauth] [% Hlb]".
     iDestruct (mono_nat_lb_own_valid with "Hauth Hlb") as %Hvalid.
@@ -100,26 +113,26 @@ Section mono_Z.
   the [mono_Z_auth_own] in the premise as long as the conclusion is introduced
   to the persistent context, for example with [iDestruct (mono_Z_lb_own_get
   with "Hauth") as "#Hfrag"]. *)
-  Lemma mono_Z_lb_own_get γ q n :
-    mono_Z_auth_own γ q n -∗ mono_Z_lb_own γ n.
+  Lemma mono_Z_lb_own_get γ dq n :
+    γ ↪●MZ{dq} n -∗ γ ↪◯MZ n.
   Proof. unseal. iIntros "[% ?]". iSplit; first done. by iApply mono_nat_lb_own_get. Qed.
 
   Lemma mono_Z_lb_own_le {γ n} n' :
     n' ≤ n →
     0 ≤ n' →
-    mono_Z_lb_own γ n -∗ mono_Z_lb_own γ n'.
+    γ ↪◯MZ n -∗ γ ↪◯MZ n'.
   Proof.
     unseal. iIntros "% % [% ?]". iSplit; first done.
     iApply mono_nat_lb_own_le; last done. lia.
   Qed.
 
   Lemma mono_Z_lb_own_0 γ :
-    ⊢ |==> mono_Z_lb_own γ 0.
+    ⊢ |==> γ ↪◯MZ 0.
   Proof. unseal. iMod mono_nat_lb_own_0 as "$". eauto. Qed.
 
   Lemma mono_Z_own_alloc n :
     0 ≤ n →
-    ⊢ |==> ∃ γ, mono_Z_auth_own γ 1 n ∗ mono_Z_lb_own γ n.
+    ⊢ |==> ∃ γ, γ ↪●MZ n ∗ γ ↪◯MZ n.
   Proof.
     unseal. intros. iMod mono_nat_own_alloc as (γ) "[??]".
     iModIntro. iExists _. iFrame. eauto.
@@ -127,12 +140,23 @@ Section mono_Z.
 
   Lemma mono_Z_own_update {γ n} n' :
     n ≤ n' →
-    mono_Z_auth_own γ 1 n ==∗ mono_Z_auth_own γ 1 n' ∗ mono_Z_lb_own γ n'.
+    γ ↪●MZ n ==∗ γ ↪●MZ n' ∗ γ ↪◯MZ n'.
   Proof.
     iIntros (?) "Hauth".
-    iAssert (mono_Z_auth_own γ 1 n') with "[> Hauth]" as "Hauth".
+    iAssert (γ ↪●MZ n') with "[> Hauth]" as "Hauth".
     { unseal. iDestruct "Hauth" as "[% Hauth]".
       iMod (mono_nat_own_update with "Hauth") as "[$ _]"; auto with lia. }
     iModIntro. iSplit; [done|]. by iApply mono_Z_lb_own_get.
+  Qed.
+
+  Lemma mono_Z_own_persist γ dq a :
+    γ ↪●MZ{dq} a ==∗ γ ↪●MZ□ a.
+  Proof.
+    unseal. iIntros "[$ Hown]". iApply mono_nat_own_persist. done.
+  Qed.
+  Lemma mono_Z_own_unpersist γ a :
+    γ ↪●MZ□ a ==∗ ∃ q, γ ↪●MZ{#q} a.
+  Proof.
+    unseal. iIntros "[$ Hown]". iApply mono_nat_own_unpersist. done.
   Qed.
 End mono_Z.
