tests/proofmode_iris.v
@@ -306,7 +306,7 @@ Section iris_tests.
   (** Make sure [iCombine] doesn't leave behind beta redexes. *)
   Check "test_iCombine_pointsto_no_beta".
   Lemma test_iCombine_ghost_var_no_beta `{!ghost_varG Σ nat} l (v : nat) q1 q2 :
-    ghost_var l q1 v -∗ ghost_var l q2 v -∗ ghost_var l (q1+q2) v.
+    l ↪VAR{#q1} v -∗ l ↪VAR{#q2} v -∗ l ↪VAR{#q1+q2} v.
   Proof.
     iIntros "H1 H2". iCombine "H1 H2" as "H". Show. done.
   Qed.
